\documentclass{article}
\usepackage{amsmath, amssymb}
\begin{document}



\begin{equation}
N^{[U]^{(1)}} = \dfrac{1}{4}\xi(\xi-1)\omega(\omega-1) 
\end{equation}
\begin{equation}
N^{[U]^{(2)}} = \dfrac{1}{4}\xi(\xi+1)\omega(\omega-1) 
\end{equation}
\begin{equation}
N^{[U]^{(3)}} = \dfrac{1}{4}\xi(\xi+1)\omega(\omega+1) 
\end{equation}
\begin{equation}
N^{[U]^{(4)}} = \dfrac{1}{4}\xi(\xi-1)\omega(\omega+1) 
\end{equation}
\begin{equation}
N^{[U]^{(5)}} = \dfrac{1}{2}(1-\xi^2)\omega(\omega-1) 
\end{equation}
\begin{equation}
N^{[U]^{(6)}} = \dfrac{1}{2}\xi(\xi+1)(1-\omega^2) 
\end{equation}
\begin{equation}
N^{[U]^{(7)}} = \dfrac{1}{2}(1-\xi^2)\omega(\omega+1) 
\end{equation}
\begin{equation}
N^{[U]^{(8)}} = \dfrac{1}{2}\xi(\xi-1)(1-\omega^2) 
\end{equation}
\begin{equation}
N^{[U]^{(9)}} = (1-\xi^2)(1-\omega^2) 
\end{equation}

\begin{equation}
N_{,\xi}^{[U]^{(1)}} = -\dfrac{1}{2}\xi\omega-\dfrac{1}{4}\omega^2+\dfrac{1}{4}\omega+\dfrac{1}{2}\xi\omega^2 
\end{equation}
\begin{equation}
N_{,\xi}^{[U]^{(2)}} = -\dfrac{1}{2}\xi\omega+\dfrac{1}{4}\omega^2-\dfrac{1}{4}\omega+\dfrac{1}{2}\xi\omega^2 
\end{equation}
\begin{equation}
N_{,\xi}^{[U]^{(3)}} = \dfrac{1}{2}\xi\omega+\dfrac{1}{4}\omega^2+\dfrac{1}{4}\omega+\dfrac{1}{2}\xi\omega^2 
\end{equation}
\begin{equation}
N_{,\xi}^{[U]^{(4)}} = \dfrac{1}{2}\xi\omega-\dfrac{1}{4}\omega^2-\dfrac{1}{4}\omega+\dfrac{1}{2}\xi\omega^2 
\end{equation}
\begin{equation}
N_{,\xi}^{[U]^{(5)}} = \xi\omega-\xi\omega^2
\end{equation}
\begin{equation}
N_{,\xi}^{[U]^{(6)}} = \xi-\xi\omega^2+\dfrac{1}{2}-\dfrac{1}{2}\omega^2
\end{equation}
\begin{equation}
N_{,\xi}^{[U]^{(7)}} = -\xi\omega-\xi\omega^2
\end{equation}
\begin{equation}
N_{,\xi}^{[U]^{(8)}} = \xi-\xi\omega^2-\dfrac{1}{2}+\dfrac{1}{2}\omega^2
\end{equation}
\begin{equation}
N_{,\xi}^{[U]^{(9)}} = -2\xi+2\xi\omega^2
\end{equation}

\begin{equation}
N_{,\omega}^{[U]^{(1)}} = -\dfrac{1}{2}\xi\omega-\dfrac{1}{4}\xi^2+\dfrac{1}{4}\xi+\dfrac{1}{2}\xi^2\omega
\end{equation}
\begin{equation}
N_{,\omega}^{[U]^{(2)}} = \dfrac{1}{2}\xi\omega-\dfrac{1}{4}\xi^2-\dfrac{1}{4}\xi+\dfrac{1}{2}\xi^2\omega
\end{equation}
\begin{equation}
N_{,\omega}^{[U]^{(3)}} = \dfrac{1}{2}\xi\omega+\dfrac{1}{4}\xi^2+\dfrac{1}{4}\xi+\dfrac{1}{2}\xi^2\omega
\end{equation}
\begin{equation}
N_{,\omega}^{[U]^{(4)}} = -\dfrac{1}{2}\xi\omega+\dfrac{1}{4}\xi^2-\dfrac{1}{4}\xi+\dfrac{1}{2}\xi^2\omega
\end{equation}
\begin{equation}
N_{,\omega}^{[U]^{(5)}} = \dfrac{1}{2}\xi^2-\dfrac{1}{2}-\xi^2\omega+\omega
\end{equation}
\begin{equation}
N_{,\omega}^{[U]^{(6)}} = -\xi^2\omega-\xi\omega
\end{equation}
\begin{equation}
N_{,\omega}^{[U]^{(7)}} =  -\dfrac{1}{2}\xi^2+\dfrac{1}{2}-\xi^2\omega+\omega
\end{equation}
\begin{equation}
N_{,\omega}^{[U]^{(8)}} = -\xi^2\omega+\xi\omega
\end{equation}
\begin{equation}
N_{,\omega}^{[U]^{(9)}} = -2\omega+2\xi^2\omega
\end{equation}

\begin{equation}
N^{[\psi]^{(1)}} = \dfrac{1}{4}(1-\xi)(1-\omega) 
\end{equation}
\begin{equation}
N^{[\psi]^{(2)}} = \dfrac{1}{4}(1+\xi)(1-\omega) 
\end{equation}
\begin{equation}
N^{[\psi]^{(3)}} = \dfrac{1}{4}(1+\xi)(1+\omega) 
\end{equation}
\begin{equation}
N^{[\psi]^{(4)}} = \dfrac{1}{4}(1-\xi)(1+\omega) 
\end{equation}

\begin{equation}
N_{,\xi}^{[\psi]^{(1)}} = \dfrac{1}{4}(-1+\omega)
\end{equation}
\begin{equation}
N_{,\xi}^{[\psi]^{(2)}} = \dfrac{1}{4}(1-\omega)
\end{equation}
\begin{equation}
N_{,\xi}^{[\psi]^{(3)}} = \dfrac{1}{4}(1+\omega)
\end{equation}
\begin{equation}
N_{,\xi}^{[\psi]^{(4)}} = \dfrac{1}{4}(-1-\omega)
\end{equation}


\begin{equation}
N_{,\omega}^{[\psi]^{(1)}} = \dfrac{1}{4}(-1+\xi)
\end{equation}
\begin{equation}
N_{,\omega}^{[\psi]^{(2)}} = \dfrac{1}{4}(-1-\xi)
\end{equation}
\begin{equation}
N_{,\omega}^{[\psi]^{(3)}} = \dfrac{1}{4}(1+\xi)
\end{equation}
\begin{equation}
N_{,\omega}^{[\psi]^{(4)}} = \dfrac{1}{4}(1-\xi)
\end{equation}


\[
u^{(e)}=
\begin{bmatrix}
u_1^{(e)}\\
u_2^{(e)}
\end{bmatrix}
=N^{[u]^{\textbf{T}}}\cdot {u}^{(e)}
\]

\[
u^{(e)}=
\begin{bmatrix}
u_1^{(1)}&u_2^{(1)}&u_1^{(2)}&u_2^{(2)}&\cdots &\cdots u_1^{(9)} u_2^{(9)}
\end{bmatrix}
\]

\[
N^{[u]^{T}}=
\begin{bmatrix}
N^{[u]^{(1)}}&0&N^{[u]^{(2)}}&0&\cdots &\cdots& N^{[u]^{(9)}}&0 \\
0&N^{[u]^{(1)}}&0&N^{[u]^{(2)}}&\cdots &\cdots& 0&N^{[u]^{(9)}}
\end{bmatrix}
\]

\[
\nabla u^{(e)}=
\begin{bmatrix}
u_{1,1}^{(e)} \\
\\
u_{1,2}^{(e)} \\
\\
u_{2,1}^{(e)} \\
\\
u_{2,2}^{(e)} 
\end{bmatrix}
=M^{[u]^{\textbf{T}}}u^{(e)}
\]

\[
M^{[u]^\textbf{T}}=
\begin{bmatrix}
N_{,1}^{[u]^{(1)}}&0&N_{,1}^{[u]^{(2)}}&0&\cdots &\cdots& N_{,1}^{[u]^{(9)}}&0 \\
0&N_{,2}^{[u]^{(1)}}&0&N_{,2}^{[u]^{(2)}}&\cdots &\cdots& 0&N_{,2}^{[u]^{(9)}} \\
N_{,1}^{[u]^{(1)}}&0&N_{,1}^{[u]^{(2)}}&0&\cdots &\cdots& N_{,1}^{[u]^{(9)}}&0 \\
0&N_{,2}^{[u]^{(1)}}&0&N_{,2}^{[u]^{(2)}}&\cdots &\cdots& 0&N_{,2}^{[u]^{(9)}}
\end{bmatrix}
\]

\[
\varepsilon^{(e)}=
\begin{bmatrix}
\varepsilon_{11}^{(e)} \\
\\
\varepsilon_{22}^{(e)}  \\
\\
\gamma_{12}^{(e)}  \\ 
\end{bmatrix}
\approx B^{[u]^{\textbf{T}}}u^{(e)}
\]

\[
B^{[u]^\textbf{T}}=
\begin{bmatrix}
N_{,1}^{[u]^{(1)}}&0&N_{,1}^{[u]^{(2)}}&0&\cdots &\cdots& N_{,1}^{[u]^{(9)}}&0 \\
0&N_{,2}^{[u]^{(1)}}&0&N_{,2}^{[u]^{(2)}}&\cdots &\cdots& 0&N_{,2}^{[u]^{(9)}} \\
N_{,2}^{[u]^{(1)}}&N_{,1}^{[u]^{(1)}}&N_{,2}^{[u]^{(2)}}&N_{,1}^{[u]^{(2)}}&\cdots &\cdots& N_{,2}^{[u]^{(9)}}&N_{,1}^{[u]^{(9)}}
\end{bmatrix}
\]

\[
\psi^{(e)}=
\begin{bmatrix}
\psi_{11}^{(e)} \\
\\
\psi_{21}^{(e)} \\
\\
\psi_{12}^{(e)} \\
\\
\psi_{22}^{(e)}
\end{bmatrix}
=N^{[\psi]^{\textbf{T}}}\psi^{(e)}
\]

\[
\psi^{(e)^{\textbf{T}}}=
\begin{bmatrix}
\psi_{(11)}^{(1)}&\psi_{(21)}^{(1)}&\psi_{(12)}^{(1)}&\psi_{(22)}^{(1)}&\cdots &\cdots& \psi_{(11)}^{(4)}&\psi_{(21)}^{(4)}&\psi_{(12)}^{(4)}&\psi_{(22)}^{(4)}
\end{bmatrix}
\]

\[
N^{[\psi]^\textbf{T}}=
\begin{bmatrix}
N^{{\psi}^{(1)}}&0&0&0&\cdots&\cdots&N^{{\psi}^{(4)}}&0&0&0 \\
0&N^{{\psi}^{(1)}}&0&0&\cdots&\cdots&0&N^{{\psi}^{(4)}}&0&0 \\
0&0&N^{{\psi}^{(1)}}&0&\cdots&\cdots&0&0&N^{{\psi}^{(4)}}&0 \\
0&0&0&N^{{\psi}^{(1)}}&\cdots&\cdots&0&0&0&N^{{\psi}^{(4)}} 
\end{bmatrix}
\]

\[
\eta^{(e)}=
\begin{bmatrix}
\eta_{111}^{(e)} \\
\\
\eta_{221}^{(e)} \\
\\
\eta_{112}^{(e)} \\
\\
\eta_{222}^{(e)} \\
\\
\phi_{1}^{(e)} \\
\\
\phi_{2}^{(e)}
\end{bmatrix}
\thickapprox B^{[\psi]^{\textbf{T}}}\psi^{(e)}
\]

\[
B^{[\psi]^\textbf{T}}=
\begin{bmatrix}
N_{,1}^{{[\psi]}^{(1)}}&0&0&0&\cdots&\cdots&N_{,1}^{{[\psi]}^{(4)}}&0&0&0 \\
0&N_{,2}^{{[\psi]}^{(1)}}&0&0&\cdots&\cdots&0&N_{,2}^{{[\psi]}^{(4)}}&0&0 \\
0&0&N_{,1}^{{[\psi]}^{(1)}}&0&\cdots&\cdots&0&0&N_{,1}^{{[\psi]}^{(4)}}&0 \\
0&0&0&N_{,2}^{{[\psi]}^{(1)}}&\cdots&\cdots&0&0&0&N_{,2}^{{[\psi]}^{(4)}} \\
N_{,2}^{{[\psi]}^{(1)}}&N_{,1}^{{[\psi]}^{(1)}}&0&0&\cdots&\cdots&N_{,2}^{{[\psi]}^{(4)}}&N_{,1}^{{[\psi]}^{(4)}}&0&0 \\
0&0&N_{,2}^{{[\psi]}^{(1)}}&N_{,1}^{{[\psi]}^{(1)}}&\cdots&\cdots&0&0&N_{,2}^{{[\psi]}^{(4)}}&N_{,1}^{{[\psi]}^{(4)}} 
\end{bmatrix}
\]


\[
\rho^{(e)}=
\begin{bmatrix}
\rho_{11}^{(e)} \\
\\
\rho_{21}^{(e)} \\
\\
\rho_{12}^{(e)} \\
\\
\rho_{22}^{(e)}
\end{bmatrix}
=N^{[\rho]^{\textbf{T}}}\rho^{(e)}
\]

\[
N^{[\rho]}=
\begin{bmatrix}
1&0&0&0 \\
\\
0&1&0&0 \\
\\
0&0&1&0 \\
\\
0&0&0&1
\end{bmatrix}
\]





\end{document}
